---
title: "HW 06 SOLUTIONS"
format: pdf
---

# Practice Problems

## 3.145
$m(t) = E(e^{ty}) = \sum_{y=0}^{n} \binom{n}{y} (pe^t)^y (1-p)^{n - y} = (pe^t + 1 - p)^n$


## 3.147

$m(t) = E(e^{ty}) = \sum_{y=1}^{\infty}pe^{ty}q^{y - 1} = pe^t\sum_{(y-1)=0}^{\infty}(qe^t)^{y - 1} = \frac{pe^t}{1 - qe^t}$

Note the second-to-last step is because $e^{ty} = (e^t)^{y - 1}e^t$ and the final step is recognizing the geometric series $\sum_{n=0}^{\infty}a^n = \frac{1}{1 - a}$.


## 3.149

This is the momentâ€“generating function for the binomial with n = 3 and p = .6.

## 3.155

Differentiate to find the necessary moments:

a. $E(Y) = \frac{7}{3}$

b. $V(Y) = E(Y^2) - [E(Y)]^2 = 6 - \left(\frac{7}{3}\right)^2 = \frac{5}{9}$

c. Since $m(t) = E(e^{tY})$, and $Y$ can only take on values $1$, $2$, and $3$ with probabilities $\frac{1}{6}$, $\frac{2}{6}$, and $\frac{3}{6}$ respectively.

# Submitted Problems

## 3.146

$m'(t) = n p e^{t}(p e^{t} + q)^{n-1}$  
At $t=0$: $E(Y) = n p$

$m''(t) = n(n-1)(pe^t + q)^{n-1}(pe^t)^2 + n(pe^t + q)^{n-1}pe^t$  
At $t=0$: $E(Y^2) = n(n-1)p^2 + np$

$V(Y) = E(Y^2) - [E(Y)]^2 = n(n-1)p^2 +np - (np)^2 = n p(1 - p)$

## 3.148

$m'(t) = \dfrac{pe^{t}}{(1 - q e^{t})^2}$  
At $t=0$: $E(Y) = \dfrac{1}{p}$

$m''(t) = \frac{(1 - qe^t)^2pe^t-2pe^t(1 - qe^t)(-qe^t)}{(1 - qe^t)^4}$.  
At $t=0$: $E(Y^2) = \dfrac{1 + q}{p^2}$

$V(Y) = E(Y^2) - [E(Y)]^2 = \dfrac{1 + q}{p^2} - \dfrac{1}{p^2} = \dfrac{q}{p^2}$

## 3.150

This is the mgf of a geometric distribution with $p = 0.3$.

## 3.158

If $m_Y(t)$ is the mgf of $Y$, then  
$m_W(t) = E(e^{tW}) = E(e^{t(aY+b)}) = E(e^{bt}e^{(at)Y}) = e^{b t} m_Y(a t)$.